pulse ht: pulse insert,delete,lookup loop invariants check with new prover! loop body's commented out for now

pulse/share/steel/examples/pulse/dice/lib/PulseHashTable.fst
@@ -60,7 +60,6 @@ let insert_loop_inv (#s:pht_sig) (b:bool)
     exists_ (fun (vcont:bool) ->
       insert_loop_inv_def b pht ht off cont k v voff vcont))
 
-// [@@expect_failure]
 ```pulse
 fn insert (#s:pht_sig) (#pht:(p:pht s{not_full p.repr})) 
           (ht:ht s) (k:s.keyt) (v:s.valt)
@@ -73,95 +72,60 @@ fn insert (#s:pht_sig) (#pht:(p:pht s{not_full p.repr}))
   let mut off = coerce_nat 0;
   let mut cont = true;
 
-  // assume_ (exists_ (fun b -> insert_loop_inv b pht ht off cont k v));
-  // with b.
-  //   assert (insert_loop_inv b pht ht off cont k v);
-  // introduce
-  //   exists (b:bool). insert_loop_inv b pht ht off cont k v
-  //   with (0 <= ht.sz && = true);
-
-  // rewrite (models s pht ht)
-  //       as (models s (match true with | true -> pht | _ -> PHT.insert pht k v) ht);
-  // fold (insert_loop_inv_def true pht ht off cont k v 0 true);
-  // rewrite (insert_loop_inv_def true pht ht off cont k v 0 true)
-  //      as (insert_loop_inv_def true pht ht off cont k v (reveal (hide 0)) (reveal (hide true)));
-  // introduce exists (voff:nat) (vcont:bool).
-  //             insert_loop_inv_def true pht ht off cont k v (reveal voff) (reveal vcont)
-  //      with 0 true;
-  // assert emp;
-  // with (voff:Ghost.erased nat) (vcont:Ghost.erased bool).
-  //   assert (insert_loop_inv_def true pht ht off cont k v (Ghost.reveal voff) (Ghost.reveal vcont));
-
-  // assert (insert_loop_inv_def true pht ht off cont k v (Ghost.reveal voff) (Ghost.reveal vcont));
-  // rewrite (insert_loop_inv_def true pht ht off cont k v (Ghost.reveal voff) (Ghost.reveal vcont))
-  //      as (insert_loop_inv_def true pht ht off cont k v
-  //           (reveal (hide (reveal (hide (reveal voff)))))
-  //           (reveal (hide (reveal (hide (reveal vcont))))));
-
-  // rewrite (insert_loop_inv_def true pht ht off cont k v (reveal (hide voff)) (reveal (hide vcont)))
-  //      as (insert_loop_inv_def true pht ht off cont k v (reveal (hide voff)) (reveal (hide vcont)))
-  //fold (insert_loop_inv true pht ht off cont k v);
-    
-
-  // rewrite (exists (voff:nat) (vcont:bool).
-  //             insert_loop_inv_def true pht ht off cont k v (reveal voff) (reveal vcont))
-  //      as (insert_loop_inv true pht ht off cont k v);
-  assume_ (insert_loop_inv true pht ht off cont k v);
-
-  assert emp;
-
-  let zz = 42;
   while (let voff = !off; let vcont = !cont; (voff <= sz && vcont = true))
-  invariant b. insert_loop_inv b pht ht off cont k v
+  invariant b. exists (voff:nat) (vcont:bool). (
+    R.pts_to off full_perm voff **
+    R.pts_to cont full_perm vcont **
+    `@(if vcont 
+      then models s pht ht
+      else models s (PHT.insert pht k v) ht) **
+    pure (
+      voff >= 0 /\ voff <= sz /\
+      b == (voff <= sz && vcont = true)
+    ))
   {
-    assume_ (exists_ (fun b -> insert_loop_inv b pht ht off cont k v));
+    admit()
     // if (off=sz) {
     // admit()
     // } else {
-      (*
-    let voff = !off;
-    let idx = coerce_us ((cidx+voff)%sz);
-    assume_ (pure (US.v idx < pht.sz)); // FIXME: can prove based on modulo calc above
-    let c = op_Array_Index ht.contents #full_perm #pht.repr idx;
-    match c {
-      Used k' v' -> { 
-        if (k' = k) {
-          op_Array_Assignment ht.contents idx (mk_used_cell k v);
-          cont := false;
-          ()
-        } else {
-          off := voff + 1;
-          ()
-        } 
-      }
-      Clean -> {
-        op_Array_Assignment ht.contents idx (mk_used_cell k v);
-        cont := false;
-        ()
-      }
-      Zombie -> {
-        let o = lookup ht k;
-        match o {
-          Some p -> {
-            op_Array_Assignment ht.contents (snd p) Zombie;
-            op_Array_Assignment ht.contents idx (mk_used_cell k v);
-          }
-          None -> { op_Array_Assignment ht.contents idx (mk_used_cell k v); }
-        };
-        cont := false;
-        ()
-      }
-      *)
-      ()
-    //};
-    };
-    fold (models s (PHT.insert pht k v) ht);
-    ()
+    // let voff = !off;
+    // let idx = coerce_us ((cidx+voff)%sz);
+    // assume_ (pure (US.v idx < pht.sz)); // FIXME: can prove based on modulo calc above
+    // let c = op_Array_Index ht.contents #full_perm #pht.repr idx;
+    // match c {
+    //   Used k' v' -> { 
+    //     if (k' = k) {
+    //       op_Array_Assignment ht.contents idx (mk_used_cell k v);
+    //       cont := false;
+    //       ()
+    //     } else {
+    //       off := voff + 1;
+    //       ()
+    //     } 
+    //   }
+    //   Clean -> {
+    //     op_Array_Assignment ht.contents idx (mk_used_cell k v);
+    //     cont := false;
+    //     ()
+    //   }
+    //   Zombie -> {
+    //     let o = lookup ht k;
+    //     match o {
+    //       Some p -> {
+    //         op_Array_Assignment ht.contents (snd p) Zombie;
+    //         op_Array_Assignment ht.contents idx (mk_used_cell k v);
+    //       }
+    //       None -> { op_Array_Assignment ht.contents idx (mk_used_cell k v); }
+    //     };
+    //     cont := false;
+    //     ()
+    //   }
+    // };};
+  }
 }
 ```
 
 
-[@@expect_failure]
 ```pulse
 fn delete (#s:pht_sig) (#pht:pht s) 
           (ht:ht s) (k:s.keyt)
@@ -171,45 +135,53 @@ fn delete (#s:pht_sig) (#pht:pht s)
   let sz = ht.sz;
   let a = ht.contents;
   let cidx = canonical_index k sz;
-  let mut off = 0;
+  let mut off = coerce_nat 0;
+  let mut cont = true;
 
   while (let voff = !off; let vcont = !cont; (voff <= sz && vcont = true))
-  invariant b. insert_loop_inv b pht ht off cont k v // FIXME: delete loop invar
+  invariant b. exists (voff:nat) (vcont:bool). (
+    R.pts_to off full_perm voff **
+    R.pts_to cont full_perm vcont **
+    `@(if vcont 
+      then models s pht ht
+      else models s (PHT.delete pht k) ht) **
+    pure (
+      voff >= 0 /\ voff <= sz /\
+      b == (voff <= sz && vcont = true)
+    ))
   {
-    if (off=sz) {
-    ()
-    } else {
-    let voff = !off;
-    let idx = coerce_us ((cidx+voff)%sz);
-    assume_ (pure (US.v idx < pht.sz)); // FIXME: can prove based on modulo calc above
-    let c = op_Array_Index ht.contents #full_perm #pht.repr idx;
-    match c {
-      Used k' v' -> { 
-        if (k' = k) {
-          op_Array_Assignment ht.contents idx Zombie;
-          cont := false;
-          ()
-        } else {
-          off := voff + 1;
-          ()
-        } 
-      }
-      Clean -> {
-        cont := false;
-        ()
-      }
-      Zombie -> { 
-        off := voff + 1;
-        () 
-      }
-    };};}
-    fold (models s (PHT.delete pht k) ht);
-    ()
+    admit()
+    // if (off=sz) {
+    // ()
+    // } else {
+    // let voff = !off;
+    // let idx = coerce_us ((cidx+voff)%sz);
+    // assume_ (pure (US.v idx < pht.sz)); // FIXME: can prove based on modulo calc above
+    // let c = op_Array_Index ht.contents #full_perm #pht.repr idx;
+    // match c {
+    //   Used k' v' -> { 
+    //     if (k' = k) {
+    //       op_Array_Assignment ht.contents idx Zombie;
+    //       cont := false;
+    //       ()
+    //     } else {
+    //       off := voff + 1;
+    //       ()
+    //     } 
+    //   }
+    //   Clean -> {
+    //     cont := false;
+    //     ()
+    //   }
+    //   Zombie -> { 
+    //     off := voff + 1;
+    //     () 
+    //   }
+    // };};
+    }
 }
 ```
 
-
-[@@expect_failure]
 ```pulse
 fn lookup (#s:pht_sig) (#pht:(p:pht s{not_full p.repr})) 
           (ht:ht s) (k:s.keyt)
@@ -222,51 +194,51 @@ fn lookup (#s:pht_sig) (#pht:(p:pht s{not_full p.repr}))
   let mut off = coerce_nat 0;
   let mut cont = true;
   let mut ret = None #(s.valt);
-  unfold (models s pht ht);
+
   while (let voff = !off; let vcont = !cont; (voff <= sz && vcont = true)) 
-  invariant b. exists (voff:nat) (vcont:bool) (o:option s.valt). (
-    A.pts_to ht.contents full_perm pht.repr **
+  invariant b. exists (voff:nat) (vcont:bool). (
+    models s pht ht **
     R.pts_to off full_perm voff **
     R.pts_to cont full_perm vcont **
-    R.pts_to ret full_perm o **
+    `@(if vcont 
+      then R.pts_to ret full_perm None
+      else R.pts_to ret full_perm (PHT.lookup pht k)) **    
     pure (
-      (if vcont=true
-        then o == None 
-        else o == PHT.lookup pht k) /\
+      voff >= 0 /\ voff <= sz /\
       b == (voff <= sz && vcont = true)
-    )
-  )
+    ))
   {
-    let voff = !off;
-    if (voff = sz) {
-      cont := false;
-      ()
-    } else {
-      let idx = coerce_us ((cidx+voff)%sz);
-      assume_ (pure (US.v idx < pht.sz)); // FIXME: can prove based on modulo calc above
-      let c = op_Array_Index ht.contents #full_perm #pht.repr idx;
-      match c {
-        Used k' v' -> { 
-          if (k' = k) {
-            cont := false;
-            ret := Some v';
-            ()
-          } else {
-            off := voff + 1;
-            () 
-          }}
-        Clean -> { 
-          cont := false;
-          ()
-         }
-        Zombie -> { 
-          off := voff + 1;
-          () 
-         }
-      };
-    };
+    admit()
+    // let voff = !off;
+    // if (voff = sz) {
+    //   cont := false;
+    //   ()
+    // } else {
+    //   let idx = coerce_us ((cidx+voff)%sz);
+    //   assume_ (pure (US.v idx < pht.sz)); // FIXME: can prove based on modulo calc above
+    //   let c = op_Array_Index ht.contents #full_perm #pht.repr idx;
+    //   match c {
+    //     Used k' v' -> { 
+    //       if (k' = k) {
+    //         cont := false;
+    //         ret := Some v';
+    //         ()
+    //       } else {
+    //         off := voff + 1;
+    //         () 
+    //       }}
+    //     Clean -> { 
+    //       cont := false;
+    //       ()
+    //      }
+    //     Zombie -> { 
+    //       off := voff + 1;
+    //       () 
+    //      }
+    // };};
   };
-  fold (models s pht ht);
-  ret
+  assert_ (R.pts_to ret full_perm (PHT.lookup pht k)); // need this assert
+  let o = !ret;
+  o
 }
 ```
